CoqOfRust/move_sui/simulations/move_bytecode_verifier/type_safety_tests/mod.v
@@ -1,11 +1,41 @@
 Require Import CoqOfRust.CoqOfRust.
 Require Import CoqOfRust.simulations.M.
 
+Require Import CoqOfRust.core.simulations.eq.
+Require Import CoqOfRust.move_sui.simulations.move_binary_format.errors.
+Require Import CoqOfRust.move_sui.simulations.move_binary_format.file_format.
+Require Import CoqOfRust.move_sui.simulations.move_binary_format.file_format_index.
+Require Import CoqOfRust.move_sui.simulations.move_bytecode_verifier.absint.
+Require Import CoqOfRust.move_sui.simulations.move_bytecode_verifier.constants.
+Require Import CoqOfRust.move_sui.simulations.move_bytecode_verifier.type_safety.
+Require Import CoqOfRust.move_sui.simulations.move_core_types.vm_status.
+
 Import simulations.M.Notations.
 
-Require CoqOfRust.move_sui.simulations.move_binary_format.file_format.
-Require CoqOfRust.move_sui.simulations.move_bytecode_verifier.absint.
-Require CoqOfRust.move_sui.simulations.move_bytecode_verifier.type_safety.
+(** ** Additional helper functions *)
+
+Definition assert_major_status
+    (result : M!? PartialVMError.t unit)
+    (status_eqb : StatusCode.t -> bool) :
+    M! unit :=
+  let! result := result in
+  match result with
+  | Result.Err error =>
+    let status := error.(PartialVMError.major_status) in
+    if status_eqb status then
+      return! tt
+    else
+      panic! "unexpected status"
+  | _ => panic! "unexpected result"
+  end.
+
+Definition assert_is_ok {Error : Set} (result : M? Error unit) : M! unit :=
+  match result with
+  | Result.Ok _ => return! tt
+  | _ => panic! "assert_is_ok failure"
+  end.
+
+(** ** Helpers for the tests from the Rust code *)
 
 (*
 fn make_module_with_ret(code: Vec<Bytecode>, return_: SignatureToken) -> CompiledModule {
@@ -40,31 +70,31 @@ fn make_module_with_ret(code: Vec<Bytecode>, return_: SignatureToken) -> Compile
 }
 *)
 Definition make_module_with_ret
-    (code : list file_format.Bytecode.t)
-    (return_ : file_format.SignatureToken.t) :
-    file_format.CompiledModule.t :=
-  let code_unit := file_format.CodeUnit.default <|
-    file_format.CodeUnit.code := code
+    (code : list Bytecode.t)
+    (return_ : SignatureToken.t) :
+    CompiledModule.t :=
+  let code_unit := CodeUnit.default <|
+    CodeUnit.code := code
   |> in
-  let fun_def := file_format.FunctionDefinition.default <|
-    file_format.FunctionDefinition.code := Some code_unit
+  let fun_def := FunctionDefinition.default <|
+    FunctionDefinition.code := Some code_unit
   |> in
   let fun_handle := {|
-    file_format.FunctionHandle.module := file_format.ModuleHandleIndex.Build_t 0;
-    file_format.FunctionHandle.name := file_format.IdentifierIndex.Build_t 0;
-    file_format.FunctionHandle.parameters := file_format.SignatureIndex.Build_t 0;
-    file_format.FunctionHandle.return_ := file_format.SignatureIndex.Build_t 1;
-    file_format.FunctionHandle.type_parameters := []
+    FunctionHandle.module := ModuleHandleIndex.Build_t 0;
+    FunctionHandle.name := IdentifierIndex.Build_t 0;
+    FunctionHandle.parameters := SignatureIndex.Build_t 0;
+    FunctionHandle.return_ := SignatureIndex.Build_t 1;
+    FunctionHandle.type_parameters := []
   |} in
-  file_format.empty_module <|
-    file_format.CompiledModule.function_handles := [fun_handle]
+  empty_module <|
+    CompiledModule.function_handles := [fun_handle]
   |> <|
-    file_format.CompiledModule.function_defs := [fun_def]
+    CompiledModule.function_defs := [fun_def]
   |> <|
-    file_format.CompiledModule.signatures := [
-      file_format.Signature.Build_t [];
-      file_format.Signature.Build_t [return_];
-      file_format.Signature.Build_t []
+    CompiledModule.signatures := [
+      Signature.Build_t [];
+      Signature.Build_t [return_];
+      Signature.Build_t []
     ]
   |>.
 
@@ -73,8 +103,519 @@ fn make_module(code: Vec<Bytecode>) -> CompiledModule {
     make_module_with_ret(code, SignatureToken::U32)
 }
 *)
-Definition make_module (code : list file_format.Bytecode.t) : file_format.CompiledModule.t :=
-  make_module_with_ret code file_format.SignatureToken.U32.
+Definition make_module (code : list Bytecode.t) : CompiledModule.t :=
+  make_module_with_ret code SignatureToken.U32.
+
+(*
+fn make_module_with_local(code: Vec<Bytecode>, signature: SignatureToken) -> CompiledModule {
+    let code_unit = CodeUnit {
+        code,
+        locals: SignatureIndex(2),
+        ..Default::default()
+    };
+
+    let fun_def = FunctionDefinition {
+        code: Some(code_unit.clone()),
+        ..Default::default()
+    };
+
+    let fun_handle = FunctionHandle {
+        module: ModuleHandleIndex(0),
+        name: IdentifierIndex(0),
+        parameters: SignatureIndex(2),
+        return_: SignatureIndex(1),
+        type_parameters: vec![],
+    };
+
+    let mut module = empty_module();
+    module.function_handles.push(fun_handle);
+    module.function_defs.push(fun_def);
+    module.signatures = vec![
+        Signature(vec![]),
+        Signature(vec![SignatureToken::U32]),
+        Signature(vec![signature]),
+    ];
+
+    module
+}
+*)
+Definition make_module_with_local
+    (code : list Bytecode.t)
+    (signature : SignatureToken.t) :
+    CompiledModule.t :=
+  let code_unit := CodeUnit.default <|
+    CodeUnit.code := code
+  |> <|
+    CodeUnit.locals := SignatureIndex.Build_t 2
+  |> in
+  let fun_def := FunctionDefinition.default <|
+    FunctionDefinition.code := Some code_unit
+  |> in
+  let fun_handle := {|
+    FunctionHandle.module := ModuleHandleIndex.Build_t 0;
+    FunctionHandle.name := IdentifierIndex.Build_t 0;
+    FunctionHandle.parameters := SignatureIndex.Build_t 2;
+    FunctionHandle.return_ := SignatureIndex.Build_t 1;
+    FunctionHandle.type_parameters := []
+  |} in
+  empty_module <|
+    CompiledModule.function_handles := [fun_handle]
+  |> <|
+    CompiledModule.function_defs := [fun_def]
+  |> <|
+    CompiledModule.signatures := [
+      Signature.Build_t [];
+      Signature.Build_t [SignatureToken.U32];
+      Signature.Build_t [signature]
+    ]
+  |>.
+
+(*
+fn add_function_with_parameters(module: &mut CompiledModule, parameters: Signature) {
+    let fun_def = FunctionDefinition {
+        code: None,
+        ..Default::default()
+    };
+
+    let fun_handle = FunctionHandle {
+        module: ModuleHandleIndex(0),
+        name: IdentifierIndex(0),
+        parameters: SignatureIndex(3),
+        return_: SignatureIndex(4),
+        type_parameters: vec![],
+    };
+
+    module.signatures.push(parameters);
+    module.signatures.push(Signature(vec![]));
+
+    module.function_handles.push(fun_handle);
+    module.function_defs.push(fun_def);
+}
+*)
+Definition add_function_with_parameters
+    (module : CompiledModule.t)
+    (parameters : Signature.t) :
+    CompiledModule.t :=
+  let fun_def := FunctionDefinition.default <|
+    FunctionDefinition.code := None
+  |> in
+  let fun_handle := {|
+    FunctionHandle.module := ModuleHandleIndex.Build_t 0;
+    FunctionHandle.name := IdentifierIndex.Build_t 0;
+    FunctionHandle.parameters := SignatureIndex.Build_t 3;
+    FunctionHandle.return_ := SignatureIndex.Build_t 4;
+    FunctionHandle.type_parameters := []
+  |} in
+  module <|
+    CompiledModule.signatures :=
+      module.(CompiledModule.signatures) ++ [parameters; Signature.Build_t []]
+  |> <|
+    CompiledModule.function_handles := module.(CompiledModule.function_handles) ++ [fun_handle]
+  |> <|
+    CompiledModule.function_defs := module.(CompiledModule.function_defs) ++ [fun_def]
+  |>.
+
+(*
+fn add_generic_function_with_parameters(
+    module: &mut CompiledModule,
+    type_parameter: SignatureToken,
+) {
+    let fun_def = FunctionDefinition {
+        code: None,
+        ..Default::default()
+    };
+
+    let fun_handle = FunctionHandle {
+        module: ModuleHandleIndex(0),
+        name: IdentifierIndex(0),
+        parameters: SignatureIndex(4),
+        return_: SignatureIndex(5),
+        type_parameters: vec![AbilitySet::PRIMITIVES],
+    };
+
+    let fun_inst = FunctionInstantiation {
+        handle: FunctionHandleIndex(1),
+        type_parameters: SignatureIndex(3),
+    };
+
+    module.signatures.push(Signature(vec![type_parameter]));
+    module
+        .signatures
+        .push(Signature(vec![SignatureToken::TypeParameter(0)]));
+    module.signatures.push(Signature(vec![]));
+
+    module.function_handles.push(fun_handle);
+    module.function_defs.push(fun_def);
+    module.function_instantiations.push(fun_inst);
+}
+*)
+Definition add_generic_function_with_parameters
+    (module : CompiledModule.t)
+    (type_parameter : SignatureToken.t) :
+    CompiledModule.t :=
+  let fun_def := FunctionDefinition.default <|
+    FunctionDefinition.code := None
+  |> in
+  let fun_handle := {|
+    FunctionHandle.module := ModuleHandleIndex.Build_t 0;
+    FunctionHandle.name := IdentifierIndex.Build_t 0;
+    FunctionHandle.parameters := SignatureIndex.Build_t 4;
+    FunctionHandle.return_ := SignatureIndex.Build_t 5;
+    FunctionHandle.type_parameters := [AbilitySet.PRIMITIVES]
+  |} in
+  let fun_inst := {|
+    FunctionInstantiation.handle := FunctionHandleIndex.Build_t 1;
+    FunctionInstantiation.type_parameters := SignatureIndex.Build_t 3
+  |} in
+  module <|
+    CompiledModule.signatures :=
+      module.(CompiledModule.signatures) ++ [
+        Signature.Build_t [type_parameter];
+        Signature.Build_t [SignatureToken.TypeParameter 0];
+        Signature.Build_t []
+      ]
+  |> <|
+    CompiledModule.function_handles := module.(CompiledModule.function_handles) ++ [fun_handle]
+  |> <|
+    CompiledModule.function_defs := module.(CompiledModule.function_defs) ++ [fun_def]
+  |>.
+
+(*
+fn add_native_struct(module: &mut CompiledModule) {
+    let struct_def = StructDefinition {
+        struct_handle: StructHandleIndex(0),
+        field_information: StructFieldInformation::Native,
+    };
+
+    let struct_handle = StructHandle {
+        module: ModuleHandleIndex(0),
+        name: IdentifierIndex(0),
+        abilities: AbilitySet::EMPTY,
+        type_parameters: vec![],
+    };
+
+    module.struct_defs.push(struct_def);
+    module.struct_handles.push(struct_handle);
+
+    module.field_handles = vec![FieldHandle {
+        owner: StructDefinitionIndex(0),
+        field: 0,
+    }];
+}
+*)
+Definition add_native_struct (module : CompiledModule.t) : CompiledModule.t :=
+  let struct_def := {|
+    StructDefinition.struct_handle := StructHandleIndex.Build_t 0;
+    StructDefinition.field_information := StructFieldInformation.Native
+  |} in
+  let struct_handle := {|
+    StructHandle.module := ModuleHandleIndex.Build_t 0;
+    StructHandle.name := IdentifierIndex.Build_t 0;
+    StructHandle.abilities := AbilitySet.EMPTY;
+    StructHandle.type_parameters := []
+  |} in
+  module <|
+    CompiledModule.struct_defs := module.(CompiledModule.struct_defs) ++ [struct_def]
+  |> <|
+    CompiledModule.struct_handles := module.(CompiledModule.struct_handles) ++ [struct_handle]
+  |> <|
+    CompiledModule.field_handles := [{|
+      FieldHandle.owner := StructDefinitionIndex.Build_t 0;
+      FieldHandle.field := 0
+    |}]
+  |>.
+
+(*
+fn add_native_struct_generic(module: &mut CompiledModule, type_parameter: SignatureToken) {
+    let struct_def = StructDefinition {
+        struct_handle: StructHandleIndex(0),
+        field_information: StructFieldInformation::Native,
+    };
+
+    let struct_handle = StructHandle {
+        module: ModuleHandleIndex(0),
+        name: IdentifierIndex(0),
+        abilities: AbilitySet::EMPTY,
+        type_parameters: vec![StructTypeParameter {
+            constraints: AbilitySet::PRIMITIVES,
+            is_phantom: false,
+        }],
+    };
+
+    module.struct_defs.push(struct_def);
+    module.struct_handles.push(struct_handle);
+    module
+        .struct_def_instantiations
+        .push(StructDefInstantiation {
+            def: StructDefinitionIndex(0),
+            type_parameters: SignatureIndex(3),
+        });
+
+    module.signatures.push(Signature(vec![type_parameter]));
+
+    module.field_handles = vec![FieldHandle {
+        owner: StructDefinitionIndex(0),
+        field: 0,
+    }];
+
+    module.field_instantiations.push(FieldInstantiation {
+        handle: FieldHandleIndex(0),
+        type_parameters: SignatureIndex(3),
+    });
+}
+*)
+Definition add_native_struct_generic
+    (module : CompiledModule.t)
+    (type_parameter : SignatureToken.t) :
+    CompiledModule.t :=
+  let struct_def := {|
+    StructDefinition.struct_handle := StructHandleIndex.Build_t 0;
+    StructDefinition.field_information := StructFieldInformation.Native
+  |} in
+  let struct_handle := {|
+    StructHandle.module := ModuleHandleIndex.Build_t 0;
+    StructHandle.name := IdentifierIndex.Build_t 0;
+    StructHandle.abilities := AbilitySet.EMPTY;
+    StructHandle.type_parameters := [{|
+      StructTypeParameter.constraints := AbilitySet.PRIMITIVES;
+      StructTypeParameter.is_phantom := false
+    |}]
+  |} in
+  module <|
+    CompiledModule.struct_defs := module.(CompiledModule.struct_defs) ++ [struct_def]
+  |> <|
+    CompiledModule.struct_handles := module.(CompiledModule.struct_handles) ++ [struct_handle]
+  |> <|
+    CompiledModule.struct_def_instantiations := module.(CompiledModule.struct_def_instantiations) ++ [{|
+      StructDefInstantiation.def := StructDefinitionIndex.Build_t 0;
+      StructDefInstantiation.type_parameters := SignatureIndex.Build_t 3
+    |}]
+  |> <|
+    CompiledModule.signatures := module.(CompiledModule.signatures) ++ [Signature.Build_t [type_parameter]]
+  |> <|
+    CompiledModule.field_handles := [{|
+      FieldHandle.owner := StructDefinitionIndex.Build_t 0;
+      FieldHandle.field := 0
+    |}]
+  |> <|
+    CompiledModule.field_instantiations := module.(CompiledModule.field_instantiations) ++ [{|
+      FieldInstantiation.handle := FieldHandleIndex.Build_t 0;
+      FieldInstantiation.type_parameters := SignatureIndex.Build_t 3
+    |}]
+  |>.
+
+(*
+fn add_simple_struct(module: &mut CompiledModule) {
+    let struct_def = StructDefinition {
+        struct_handle: StructHandleIndex(0),
+        field_information: StructFieldInformation::Declared(vec![
+            FieldDefinition {
+                name: IdentifierIndex(5),
+                signature: TypeSignature(SignatureToken::U32),
+            },
+            FieldDefinition {
+                name: IdentifierIndex(6),
+                signature: TypeSignature(SignatureToken::Bool),
+            },
+        ]),
+    };
+
+    let struct_handle = StructHandle {
+        module: ModuleHandleIndex(0),
+        name: IdentifierIndex(0),
+        abilities: AbilitySet::EMPTY,
+        type_parameters: vec![],
+    };
+
+    module.struct_defs.push(struct_def);
+    module.struct_handles.push(struct_handle);
+
+    module.field_handles = vec![
+        FieldHandle {
+            owner: StructDefinitionIndex(0),
+            field: 0,
+        },
+        FieldHandle {
+            owner: StructDefinitionIndex(0),
+            field: 1,
+        },
+    ];
+}
+*)
+Definition add_simple_struct (module : CompiledModule.t) : CompiledModule.t :=
+  let struct_def := {|
+    StructDefinition.struct_handle := StructHandleIndex.Build_t 0;
+    StructDefinition.field_information := StructFieldInformation.Declared [
+      {|
+        FieldDefinition.name := IdentifierIndex.Build_t 5;
+        FieldDefinition.signature := TypeSignature.Build_t (SignatureToken.U32)
+      |};
+      {|
+        FieldDefinition.name := IdentifierIndex.Build_t 6;
+        FieldDefinition.signature := TypeSignature.Build_t (SignatureToken.Bool)
+      |}
+    ]
+  |} in
+  let struct_handle := {|
+    StructHandle.module := ModuleHandleIndex.Build_t 0;
+    StructHandle.name := IdentifierIndex.Build_t 0;
+    StructHandle.abilities := AbilitySet.EMPTY;
+    StructHandle.type_parameters := []
+  |} in
+  module <|
+    CompiledModule.struct_defs := module.(CompiledModule.struct_defs) ++ [struct_def]
+  |> <|
+    CompiledModule.struct_handles := module.(CompiledModule.struct_handles) ++ [struct_handle]
+  |> <|
+    CompiledModule.field_handles := [
+      {|
+        FieldHandle.owner := StructDefinitionIndex.Build_t 0;
+        FieldHandle.field := 0
+      |};
+      {|
+        FieldHandle.owner := StructDefinitionIndex.Build_t 0;
+        FieldHandle.field := 1
+      |}
+    ]
+  |>.
+
+(*
+fn add_simple_struct_with_abilities(module: &mut CompiledModule, abilities: AbilitySet) {
+    let struct_def = StructDefinition {
+        struct_handle: StructHandleIndex(0),
+        field_information: StructFieldInformation::Declared(vec![FieldDefinition {
+            name: IdentifierIndex(5),
+            signature: TypeSignature(SignatureToken::U32),
+        }]),
+    };
+
+    let struct_handle = StructHandle {
+        module: ModuleHandleIndex(0),
+        name: IdentifierIndex(0),
+        abilities: abilities,
+        type_parameters: vec![],
+    };
+
+    module.struct_defs.push(struct_def);
+    module.struct_handles.push(struct_handle);
+}
+*)
+Definition add_simple_struct_with_abilities
+    (module : CompiledModule.t)
+    (abilities : AbilitySet.t) :
+    CompiledModule.t :=
+  let struct_def := {|
+    StructDefinition.struct_handle := StructHandleIndex.Build_t 0;
+    StructDefinition.field_information := StructFieldInformation.Declared [
+      {|
+        FieldDefinition.name := IdentifierIndex.Build_t 5;
+        FieldDefinition.signature := TypeSignature.Build_t (SignatureToken.U32)
+      |}
+    ]
+  |} in
+  let struct_handle := {|
+    StructHandle.module := ModuleHandleIndex.Build_t 0;
+    StructHandle.name := IdentifierIndex.Build_t 0;
+    StructHandle.abilities := abilities;
+    StructHandle.type_parameters := []
+  |} in
+  module <|
+    CompiledModule.struct_defs := module.(CompiledModule.struct_defs) ++ [struct_def]
+  |> <|
+    CompiledModule.struct_handles := module.(CompiledModule.struct_handles) ++ [struct_handle]
+  |>.
+
+(*
+fn add_simple_struct_generic_with_abilities(
+    module: &mut CompiledModule,
+    abilities: AbilitySet,
+    type_parameter: SignatureToken,
+) {
+    let struct_def = StructDefinition {
+        struct_handle: StructHandleIndex(0),
+        field_information: StructFieldInformation::Declared(vec![FieldDefinition {
+            name: IdentifierIndex(5),
+            signature: TypeSignature(SignatureToken::TypeParameter(0)),
+        }]),
+    };
+
+    let struct_handle = StructHandle {
+        module: ModuleHandleIndex(0),
+        name: IdentifierIndex(0),
+        abilities: abilities,
+        type_parameters: vec![StructTypeParameter {
+            constraints: AbilitySet::PRIMITIVES,
+            is_phantom: false,
+        }],
+    };
+
+    module.struct_defs.push(struct_def);
+    module.struct_handles.push(struct_handle);
+    module
+        .struct_def_instantiations
+        .push(StructDefInstantiation {
+            def: StructDefinitionIndex(0),
+            type_parameters: SignatureIndex(3),
+        });
+
+    module.signatures.push(Signature(vec![type_parameter]));
+
+    module.field_handles = vec![FieldHandle {
+        owner: StructDefinitionIndex(0),
+        field: 0,
+    }];
+
+    module.field_instantiations.push(FieldInstantiation {
+        handle: FieldHandleIndex(0),
+        type_parameters: SignatureIndex(3),
+    });
+}
+*)
+Definition add_simple_struct_generic_with_abilities
+    (module : CompiledModule.t)
+    (abilities : AbilitySet.t)
+    (type_parameter : SignatureToken.t) :
+    CompiledModule.t :=
+  let struct_def := {|
+    StructDefinition.struct_handle := StructHandleIndex.Build_t 0;
+    StructDefinition.field_information := StructFieldInformation.Declared [
+      {|
+        FieldDefinition.name := IdentifierIndex.Build_t 5;
+        FieldDefinition.signature := TypeSignature.Build_t (SignatureToken.TypeParameter 0)
+      |}
+    ]
+  |} in
+  let struct_handle := {|
+    StructHandle.module := ModuleHandleIndex.Build_t 0;
+    StructHandle.name := IdentifierIndex.Build_t 0;
+    StructHandle.abilities := abilities;
+    StructHandle.type_parameters := [{|
+      StructTypeParameter.constraints := AbilitySet.PRIMITIVES;
+      StructTypeParameter.is_phantom := false
+    |}]
+  |} in
+  module <|
+    CompiledModule.struct_defs := module.(CompiledModule.struct_defs) ++ [struct_def]
+  |> <|
+    CompiledModule.struct_handles := module.(CompiledModule.struct_handles) ++ [struct_handle]
+  |> <|
+    CompiledModule.struct_def_instantiations := module.(CompiledModule.struct_def_instantiations) ++ [{|
+      StructDefInstantiation.def := StructDefinitionIndex.Build_t 0;
+      StructDefInstantiation.type_parameters := SignatureIndex.Build_t 3
+    |}]
+  |> <|
+    CompiledModule.signatures := module.(CompiledModule.signatures) ++ [Signature.Build_t [type_parameter]]
+  |> <|
+    CompiledModule.field_handles := [{|
+      FieldHandle.owner := StructDefinitionIndex.Build_t 0;
+      FieldHandle.field := 0
+    |}]
+  |> <|
+    CompiledModule.field_instantiations := module.(CompiledModule.field_instantiations) ++ [{|
+      FieldInstantiation.handle := FieldHandleIndex.Build_t 0;
+      FieldInstantiation.type_parameters := SignatureIndex.Build_t 3
+    |}]
+  |>.
 
 (*
 fn get_fun_context(module: &CompiledModule) -> FunctionContext {
@@ -86,24 +627,26 @@ fn get_fun_context(module: &CompiledModule) -> FunctionContext {
     )
 }
 *)
-Definition get_fun_context (module : file_format.CompiledModule.t) :
-    M! type_safety.FunctionContext.t :=
+Definition get_fun_context (module : CompiledModule.t) :
+    M! FunctionContext.t :=
   match
-    module.(file_format.CompiledModule.function_defs),
-    module.(file_format.CompiledModule.function_handles)
+    module.(CompiledModule.function_defs),
+    module.(CompiledModule.function_handles)
   with
   | function_def :: _, function_handle :: _ =>
-    match function_def.(file_format.FunctionDefinition.code) with
+    match function_def.(FunctionDefinition.code) with
     | Some code =>
-      absint.Impl_FunctionContext.new
+      Impl_FunctionContext.new
         module
-        (file_format.FunctionDefinitionIndex.Build_t 0)
+        (FunctionDefinitionIndex.Build_t 0)
         code
         function_handle
     | None => panic! "function def does not have code"
     end
   | _, _ => panic! "cannot get the first function def/handle"
   end.
+
+(** **  The tests themselves *)
 
 (*
 #[test]
@@ -117,18 +660,18 @@ fn test_br_true_false_correct_type() {
     }
 }
 *)
-Definition test_br_true_false_correct_type (instr : file_format.Bytecode.t) :
-    M!? errors.PartialVMError.t unit :=
-  let code := [file_format.Bytecode.LdTrue; instr] in
+Definition test_br_true_false_correct_type (instr : Bytecode.t) :
+    M!? PartialVMError.t unit :=
+  let code := [Bytecode.LdTrue; instr] in
   let module := make_module code in
   let! fun_context := get_fun_context module in
-  type_safety.verify module fun_context.
+  verify module fun_context.
 
 Goal List.Forall
   (fun instr => test_br_true_false_correct_type instr = return!? tt)
   [
-    file_format.Bytecode.BrTrue 0;
-    file_format.Bytecode.BrFalse 0
+    Bytecode.BrTrue 0;
+    Bytecode.BrFalse 0
   ].
 Proof.
   repeat constructor.
@@ -149,26 +692,24 @@ fn test_br_true_false_wrong_type() {
     }
 }
 *)
-Definition test_br_true_false_wrong_type (instr : file_format.Bytecode.t) : M! unit :=
-  let code := [file_format.Bytecode.LdU32 0; instr] in
+Definition test_br_true_false_wrong_type (instr : Bytecode.t) : M! unit :=
+  let code := [Bytecode.LdU32 0; instr] in
   let module := make_module code in
   let! fun_context := get_fun_context module in
-  let! result := type_safety.verify module fun_context in
-  match result with
-  | Result.Err error =>
-    let status := error.(errors.PartialVMError.major_status) in
-    match status with
-    | errors.StatusCode.BR_TYPE_MISMATCH_ERROR => return! tt
-    | _ => panic! "unexpected status"
-    end
-  | _ => panic! "unexpected result"
-  end.
+  assert_major_status
+    (verify module fun_context)
+    (fun status =>
+      match status with
+      | StatusCode.BR_TYPE_MISMATCH_ERROR => true
+      | _ => false
+      end
+    ).
 
 Goal List.Forall
   (fun instr => test_br_true_false_wrong_type instr = return! tt)
   [
-    file_format.Bytecode.BrTrue 0;
-    file_format.Bytecode.BrFalse 0
+    Bytecode.BrTrue 0;
+    Bytecode.BrFalse 0
   ].
 Proof.
   repeat constructor.
@@ -186,11 +727,11 @@ fn test_br_true_false_no_arg() {
     }
 }
 *)
-Definition test_br_true_false_no_arg (instr : file_format.Bytecode.t) : M!? _ unit :=
+Definition test_br_true_false_no_arg (instr : Bytecode.t) : M!? _ unit :=
   let code := [instr] in
   let module := make_module code in
   let! fun_context := get_fun_context module in
-  type_safety.verify module fun_context.
+  verify module fun_context.
 
 Goal List.Forall
   (fun instr =>
@@ -198,9 +739,1594 @@ Goal List.Forall
     test_br_true_false_no_arg instr = panic! error
   )
   [
-    file_format.Bytecode.BrTrue 0;
-    file_format.Bytecode.BrFalse 0
+    Bytecode.BrTrue 0;
+    Bytecode.BrFalse 0
   ].
 Proof.
   repeat econstructor.
 Qed.
+
+(*
+#[test]
+fn test_abort_correct_type() {
+    let code = vec![Bytecode::LdU64(0), Bytecode::Abort];
+    let module = make_module(code);
+    let fun_context = get_fun_context(&module);
+    let result = type_safety::verify(&module, &fun_context, &mut DummyMeter);
+    assert!(result.is_ok());
+}
+*)
+Definition test_abort_correct_type : M!? PartialVMError.t unit :=
+  let code := [Bytecode.LdU64 0; Bytecode.Abort] in
+  let module := make_module code in
+  let! fun_context := get_fun_context module in
+  verify module fun_context.
+
+Goal test_abort_correct_type = return!? tt.
+Proof. reflexivity. Qed.
+
+(*
+#[test]
+fn test_abort_wrong_type() {
+    let code = vec![Bytecode::LdU32(0), Bytecode::Abort];
+    let module = make_module(code);
+    let fun_context = get_fun_context(&module);
+    let result = type_safety::verify(&module, &fun_context, &mut DummyMeter);
+    assert_eq!(
+        result.unwrap_err().major_status(),
+        StatusCode::ABORT_TYPE_MISMATCH_ERROR
+    );
+}
+*)
+Definition test_abort_wrong_type : M! unit :=
+  let code := [Bytecode.LdU32 0; Bytecode.Abort] in
+  let module := make_module code in
+  let! fun_context := get_fun_context module in
+  assert_major_status
+    (verify module fun_context)
+    (fun status =>
+      match status with
+      | StatusCode.ABORT_TYPE_MISMATCH_ERROR => true
+      | _ => false
+      end
+    ).
+
+Goal test_abort_wrong_type = return! tt.
+Proof. reflexivity. Qed.
+
+(*
+#[test]
+#[should_panic]
+fn test_abort_no_arg() {
+    let code = vec![Bytecode::Abort];
+    let module = make_module(code);
+    let fun_context = get_fun_context(&module);
+    let _result = type_safety::verify(&module, &fun_context, &mut DummyMeter);
+}
+*)
+Definition test_abort_no_arg : M!? _ unit :=
+  let code := [Bytecode.Abort] in
+  let module := make_module code in
+  let! fun_context := get_fun_context module in
+  verify module fun_context.
+
+Goal
+  exists (Error : Set) (error : Error),
+  test_abort_no_arg = panic! error.
+Proof. repeat eexists. Qed.
+
+(*
+#[test]
+fn test_cast_correct_type() {
+    for instr in vec![
+        Bytecode::CastU8,
+        Bytecode::CastU16,
+        Bytecode::CastU32,
+        Bytecode::CastU64,
+        Bytecode::CastU128,
+        Bytecode::CastU256,
+    ] {
+        let code = vec![Bytecode::LdU64(0), instr];
+        let module = make_module(code);
+        let fun_context = get_fun_context(&module);
+        let result = type_safety::verify(&module, &fun_context, &mut DummyMeter);
+        assert!(result.is_ok());
+    }
+}
+*)
+Definition test_cast_correct_type
+    (instr : Bytecode.t) :
+    M!? PartialVMError.t unit :=
+  let code := [Bytecode.LdU64 0; instr] in
+  let module := make_module code in
+  let! fun_context := get_fun_context module in
+  verify module fun_context.
+
+Goal List.Forall
+  (fun instr => test_cast_correct_type instr = return!? tt)
+  [
+    Bytecode.CastU8;
+    Bytecode.CastU16;
+    Bytecode.CastU32;
+    Bytecode.CastU64;
+    Bytecode.CastU128;
+    Bytecode.CastU256
+  ].
+Proof. repeat constructor. Qed.
+
+(*
+#[test]
+fn test_cast_wrong_type() {
+    for instr in vec![
+        Bytecode::CastU8,
+        Bytecode::CastU16,
+        Bytecode::CastU32,
+        Bytecode::CastU64,
+        Bytecode::CastU128,
+        Bytecode::CastU256,
+    ] {
+        let code = vec![Bytecode::LdTrue, instr];
+        let module = make_module(code);
+        let fun_context = get_fun_context(&module);
+        let result = type_safety::verify(&module, &fun_context, &mut DummyMeter);
+        assert_eq!(
+            result.unwrap_err().major_status(),
+            StatusCode::INTEGER_OP_TYPE_MISMATCH_ERROR
+        );
+    }
+}
+*)
+Definition test_cast_wrong_type
+    (instr : Bytecode.t) :
+    M! unit :=
+  let code := [Bytecode.LdTrue; instr] in
+  let module := make_module code in
+  let! fun_context := get_fun_context module in
+  assert_major_status
+    (verify module fun_context)
+    (fun status =>
+      match status with
+      | StatusCode.INTEGER_OP_TYPE_MISMATCH_ERROR => true
+      | _ => false
+      end
+    ).
+
+Goal List.Forall
+  (fun instr => test_cast_wrong_type instr = return! tt)
+  [
+    Bytecode.CastU8;
+    Bytecode.CastU16;
+    Bytecode.CastU32;
+    Bytecode.CastU64;
+    Bytecode.CastU128;
+    Bytecode.CastU256
+  ].
+Proof. repeat constructor. Qed.
+
+(*
+#[test]
+#[should_panic]
+fn test_cast_no_arg() {
+    for instr in vec![
+        Bytecode::CastU8,
+        Bytecode::CastU16,
+        Bytecode::CastU32,
+        Bytecode::CastU64,
+        Bytecode::CastU128,
+        Bytecode::CastU256,
+    ] {
+        let code = vec![instr];
+        let module = make_module(code);
+        let fun_context = get_fun_context(&module);
+        let _result = type_safety::verify(&module, &fun_context, &mut DummyMeter);
+    }
+}
+*)
+Definition test_cast_no_arg
+    (instr : Bytecode.t) :
+    M!? _ unit :=
+  let code := [instr] in
+  let module := make_module code in
+  let! fun_context := get_fun_context module in
+  verify module fun_context.
+
+Goal List.Forall
+  (fun instr =>
+    exists (Error : Set) (error : Error),
+    test_cast_no_arg instr = panic! error
+  )
+  [
+    Bytecode.CastU8;
+    Bytecode.CastU16;
+    Bytecode.CastU32;
+    Bytecode.CastU64;
+    Bytecode.CastU128;
+    Bytecode.CastU256
+  ].
+Proof. repeat econstructor. Qed.
+
+(*
+#[test]
+fn test_arithmetic_correct_types() {
+    for instr in vec![
+        Bytecode::Add,
+        Bytecode::Sub,
+        Bytecode::Mul,
+        Bytecode::Mod,
+        Bytecode::Div,
+        Bytecode::BitOr,
+        Bytecode::BitAnd,
+        Bytecode::Xor,
+    ] {
+        for push_ty_instr in vec![
+            Bytecode::LdU8(42),
+            Bytecode::LdU16(257),
+            Bytecode::LdU32(89),
+            Bytecode::LdU64(94),
+            Bytecode::LdU128(Box::new(9999)),
+            Bytecode::LdU256(Box::new(U256::from(745_u32))),
+        ] {
+            let code = vec![push_ty_instr.clone(), push_ty_instr.clone(), instr.clone()];
+            let module = make_module(code);
+            let fun_context = get_fun_context(&module);
+            let result = type_safety::verify(&module, &fun_context, &mut DummyMeter);
+            assert!(result.is_ok());
+        }
+    }
+}
+*)
+Definition test_arithmetic_correct_types
+    (instr push_ty_instr : Bytecode.t) :
+    M!? PartialVMError.t unit :=
+  let code := [push_ty_instr; push_ty_instr; instr] in
+  let module := make_module code in
+  let! fun_context := get_fun_context module in
+  verify module fun_context.
+
+Goal List.Forall
+  (fun instr =>
+    List.Forall
+      (fun push_ty_instr =>
+        test_arithmetic_correct_types instr push_ty_instr = return!? tt
+      )
+      [
+        Bytecode.LdU8 42;
+        Bytecode.LdU16 257;
+        Bytecode.LdU32 89;
+        Bytecode.LdU64 94;
+        Bytecode.LdU128 9999;
+        Bytecode.LdU256 745
+      ]
+  )
+  [
+    Bytecode.Add;
+    Bytecode.Sub;
+    Bytecode.Mul;
+    Bytecode.Mod;
+    Bytecode.Div;
+    Bytecode.BitOr;
+    Bytecode.BitAnd;
+    Bytecode.Xor
+  ].
+Proof.
+  repeat constructor.
+Qed.
+
+(*
+#[test]
+fn test_arithmetic_mismatched_types() {
+    for instr in vec![
+        Bytecode::Add,
+        Bytecode::Sub,
+        Bytecode::Mul,
+        Bytecode::Mod,
+        Bytecode::Div,
+        Bytecode::BitOr,
+        Bytecode::BitAnd,
+        Bytecode::Xor,
+    ] {
+        let code = vec![Bytecode::LdU8(42), Bytecode::LdU64(94), instr];
+        let module = make_module(code);
+        let fun_context = get_fun_context(&module);
+        let result = type_safety::verify(&module, &fun_context, &mut DummyMeter);
+        assert_eq!(
+            result.unwrap_err().major_status(),
+            StatusCode::INTEGER_OP_TYPE_MISMATCH_ERROR
+        );
+    }
+}
+*)
+Definition test_arithmetic_mismatched_types
+    (instr : Bytecode.t) :
+    M! unit :=
+  let code := [Bytecode.LdU8 42; Bytecode.LdU64 94; instr] in
+  let module := make_module code in
+  let! fun_context := get_fun_context module in
+  assert_major_status
+    (verify module fun_context)
+    (fun status =>
+      match status with
+      | StatusCode.INTEGER_OP_TYPE_MISMATCH_ERROR => true
+      | _ => false
+      end
+    ).
+
+Goal List.Forall
+  (fun instr => test_arithmetic_mismatched_types instr = return! tt)
+  [
+    Bytecode.Add;
+    Bytecode.Sub;
+    Bytecode.Mul;
+    Bytecode.Mod;
+    Bytecode.Div;
+    Bytecode.BitOr;
+    Bytecode.BitAnd;
+    Bytecode.Xor
+  ].
+Proof.
+  repeat constructor.
+Qed.
+
+(*
+#[test]
+fn test_arithmetic_wrong_type() {
+    for instr in vec![
+        Bytecode::Add,
+        Bytecode::Sub,
+        Bytecode::Mul,
+        Bytecode::Mod,
+        Bytecode::Div,
+        Bytecode::BitOr,
+        Bytecode::BitAnd,
+        Bytecode::Xor,
+    ] {
+        let code = vec![Bytecode::LdTrue, Bytecode::LdU64(94), instr.clone()];
+        let module = make_module(code);
+        let fun_context = get_fun_context(&module);
+        let result = type_safety::verify(&module, &fun_context, &mut DummyMeter);
+        assert_eq!(
+            result.unwrap_err().major_status(),
+            StatusCode::INTEGER_OP_TYPE_MISMATCH_ERROR
+        );
+
+        let code = vec![Bytecode::LdU32(94), Bytecode::LdFalse, instr.clone()];
+        let module = make_module(code);
+        let fun_context = get_fun_context(&module);
+        let result = type_safety::verify(&module, &fun_context, &mut DummyMeter);
+        assert_eq!(
+            result.unwrap_err().major_status(),
+            StatusCode::INTEGER_OP_TYPE_MISMATCH_ERROR
+        );
+    }
+}
+*)
+Definition test_arithmetic_wrong_type
+    (instr : Bytecode.t) :
+    M! unit :=
+  let code := [Bytecode.LdTrue; Bytecode.LdU64 94; instr] in
+  let module := make_module code in
+  let! fun_context := get_fun_context module in
+  let result := verify module fun_context in
+  do! assert_major_status
+    result
+    (fun status =>
+      match status with
+      | StatusCode.INTEGER_OP_TYPE_MISMATCH_ERROR => true
+      | _ => false
+      end
+    ) in
+  let code := [Bytecode.LdU32 94; Bytecode.LdFalse; instr] in
+  let module := make_module code in
+  let! fun_context := get_fun_context module in
+  let result := verify module fun_context in
+  assert_major_status
+    result
+    (fun status =>
+      match status with
+      | StatusCode.INTEGER_OP_TYPE_MISMATCH_ERROR => true
+      | _ => false
+      end
+    ).
+
+Goal List.Forall
+  (fun instr => test_arithmetic_wrong_type instr = return! tt)
+  [
+    Bytecode.Add;
+    Bytecode.Sub;
+    Bytecode.Mul;
+    Bytecode.Mod;
+    Bytecode.Div;
+    Bytecode.BitOr;
+    Bytecode.BitAnd;
+    Bytecode.Xor
+  ].
+Proof.
+  repeat constructor.
+Qed.
+
+(*
+#[test]
+#[should_panic]
+fn test_arithmetic_too_few_args() {
+    for instr in vec![
+        Bytecode::Add,
+        Bytecode::Sub,
+        Bytecode::Mul,
+        Bytecode::Mod,
+        Bytecode::Div,
+        Bytecode::BitOr,
+        Bytecode::BitAnd,
+        Bytecode::Xor,
+    ] {
+        let code = vec![Bytecode::LdU16(42), instr.clone()];
+        let module = make_module(code);
+        let fun_context = get_fun_context(&module);
+        let _result = type_safety::verify(&module, &fun_context, &mut DummyMeter);
+    }
+}
+*)
+Definition test_arithmetic_too_few_args
+    (instr : Bytecode.t) :
+    M!? _ unit :=
+  let code := [Bytecode.LdU16 42; instr] in
+  let module := make_module code in
+  let! fun_context := get_fun_context module in
+  verify module fun_context.
+
+Goal List.Forall
+  (fun instr =>
+    exists (Error : Set) (error : Error),
+    test_arithmetic_too_few_args instr = panic! error
+  )
+  [
+    Bytecode.Add;
+    Bytecode.Sub;
+    Bytecode.Mul;
+    Bytecode.Mod;
+    Bytecode.Div;
+    Bytecode.BitOr;
+    Bytecode.BitAnd;
+    Bytecode.Xor
+  ].
+Proof. repeat econstructor. Qed.
+
+(*
+#[test]
+#[should_panic]
+fn test_arithmetic_no_args() {
+    for instr in vec![
+        Bytecode::Add,
+        Bytecode::Sub,
+        Bytecode::Mul,
+        Bytecode::Mod,
+        Bytecode::Div,
+        Bytecode::BitOr,
+        Bytecode::BitAnd,
+        Bytecode::Xor,
+    ] {
+        let code = vec![instr.clone()];
+        let module = make_module(code);
+        let fun_context = get_fun_context(&module);
+        let _result = type_safety::verify(&module, &fun_context, &mut DummyMeter);
+    }
+}
+*)
+Definition test_arithmetic_no_args
+    (instr : Bytecode.t) :
+    M!? _ unit :=
+  let code := [instr] in
+  let module := make_module code in
+  let! fun_context := get_fun_context module in
+  verify module fun_context.
+
+Goal List.Forall
+  (fun instr =>
+    exists (Error : Set) (error : Error),
+    test_arithmetic_no_args instr = panic! error
+  )
+  [
+    Bytecode.Add;
+    Bytecode.Sub;
+    Bytecode.Mul;
+    Bytecode.Mod;
+    Bytecode.Div;
+    Bytecode.BitOr;
+    Bytecode.BitAnd;
+    Bytecode.Xor
+  ].
+Proof. repeat econstructor. Qed.
+
+(*
+#[test]
+fn test_shl_shr_correct_types() {
+    for instr in vec![Bytecode::Shl, Bytecode::Shr] {
+        for push_ty_instr in vec![
+            Bytecode::LdU8(42),
+            Bytecode::LdU16(257),
+            Bytecode::LdU32(89),
+            Bytecode::LdU64(94),
+            Bytecode::LdU128(Box::new(9999)),
+            Bytecode::LdU256(Box::new(U256::from(745_u32))),
+        ] {
+            let code = vec![push_ty_instr.clone(), Bytecode::LdU8(2), instr.clone()];
+            let module = make_module(code);
+            let fun_context = get_fun_context(&module);
+            let result = type_safety::verify(&module, &fun_context, &mut DummyMeter);
+            assert!(result.is_ok());
+        }
+    }
+}
+*)
+Definition test_shl_shr_correct_types
+    (instr push_ty_instr : Bytecode.t) :
+    M!? PartialVMError.t unit :=
+  let code := [push_ty_instr; Bytecode.LdU8 2; instr] in
+  let module := make_module code in
+  let! fun_context := get_fun_context module in
+  verify module fun_context.
+
+Goal List.Forall
+  (fun instr =>
+    List.Forall
+      (fun push_ty_instr =>
+        test_shl_shr_correct_types instr push_ty_instr = return!? tt
+      )
+      [
+        Bytecode.LdU8 42;
+        Bytecode.LdU16 257;
+        Bytecode.LdU32 89;
+        Bytecode.LdU64 94;
+        Bytecode.LdU128 9999;
+        Bytecode.LdU256 745
+      ]
+  )
+  [
+    Bytecode.Shl;
+    Bytecode.Shr
+  ].
+Proof.
+  repeat constructor.
+Qed.
+
+(*
+#[test]
+fn test_shl_shr_first_operand_wrong_type() {
+    for instr in vec![Bytecode::Shl, Bytecode::Shr] {
+        let code = vec![Bytecode::LdTrue, Bytecode::LdU8(2), instr.clone()];
+        let module = make_module(code);
+        let fun_context = get_fun_context(&module);
+        let result = type_safety::verify(&module, &fun_context, &mut DummyMeter);
+        assert_eq!(
+            result.unwrap_err().major_status(),
+            StatusCode::INTEGER_OP_TYPE_MISMATCH_ERROR
+        );
+    }
+}
+*)
+Definition test_shl_shr_first_operand_wrong_type
+    (instr : Bytecode.t) :
+    M! unit :=
+  let code := [Bytecode.LdTrue; Bytecode.LdU8 2; instr] in
+  let module := make_module code in
+  let! fun_context := get_fun_context module in
+  assert_major_status
+    (verify module fun_context)
+    (fun status =>
+      match status with
+      | StatusCode.INTEGER_OP_TYPE_MISMATCH_ERROR => true
+      | _ => false
+      end
+    ).
+
+Goal List.Forall
+  (fun instr => test_shl_shr_first_operand_wrong_type instr = return! tt)
+  [
+    Bytecode.Shl;
+    Bytecode.Shr
+  ].
+Proof.
+  repeat constructor.
+Qed.
+
+(*
+#[test]
+fn test_shl_shr_second_operand_wrong_type() {
+    for instr in vec![Bytecode::Shl, Bytecode::Shr] {
+        let code = vec![Bytecode::LdU32(42), Bytecode::LdU16(2), instr.clone()];
+        let module = make_module(code);
+        let fun_context = get_fun_context(&module);
+        let result = type_safety::verify(&module, &fun_context, &mut DummyMeter);
+        assert_eq!(
+            result.unwrap_err().major_status(),
+            StatusCode::INTEGER_OP_TYPE_MISMATCH_ERROR
+        );
+    }
+}
+*)
+Definition test_shl_shr_second_operand_wrong_type
+    (instr : Bytecode.t) :
+    M! unit :=
+  let code := [Bytecode.LdU32 42; Bytecode.LdU16 2; instr] in
+  let module := make_module code in
+  let! fun_context := get_fun_context module in
+  assert_major_status
+    (verify module fun_context)
+    (fun status =>
+      match status with
+      | StatusCode.INTEGER_OP_TYPE_MISMATCH_ERROR => true
+      | _ => false
+      end
+    ).
+
+Goal List.Forall
+  (fun instr => test_shl_shr_second_operand_wrong_type instr = return! tt)
+  [
+    Bytecode.Shl;
+    Bytecode.Shr
+  ].
+Proof.
+  repeat constructor.
+Qed.
+
+(*
+#[test]
+#[should_panic]
+fn test_shl_shr_too_few_args() {
+    for instr in vec![Bytecode::Shl, Bytecode::Shr] {
+        let code = vec![Bytecode::LdU16(42), instr.clone()];
+        let module = make_module(code);
+        let fun_context = get_fun_context(&module);
+        let _result = type_safety::verify(&module, &fun_context, &mut DummyMeter);
+    }
+}
+*)
+Definition test_shl_shr_too_few_args
+    (instr : Bytecode.t) :
+    M!? _ unit :=
+  let code := [Bytecode.LdU16 42; instr] in
+  let module := make_module code in
+  let! fun_context := get_fun_context module in
+  verify module fun_context.
+
+Goal List.Forall
+  (fun instr =>
+    exists (Error : Set) (error : Error),
+    test_shl_shr_too_few_args instr = panic! error
+  )
+  [
+    Bytecode.Shl;
+    Bytecode.Shr
+  ].
+Proof. repeat econstructor. Qed.
+
+(*
+#[test]
+#[should_panic]
+fn test_shl_shr_no_args() {
+    for instr in vec![Bytecode::Shl, Bytecode::Shr] {
+        let code = vec![instr.clone()];
+        let module = make_module(code);
+        let fun_context = get_fun_context(&module);
+        let _result = type_safety::verify(&module, &fun_context, &mut DummyMeter);
+    }
+}
+*)
+Definition test_shl_shr_no_args
+    (instr : Bytecode.t) :
+    M!? _ unit :=
+  let code := [instr] in
+  let module := make_module code in
+  let! fun_context := get_fun_context module in
+  verify module fun_context.
+
+Goal List.Forall
+  (fun instr =>
+    exists (Error : Set) (error : Error),
+    test_shl_shr_no_args instr = panic! error
+  )
+  [
+    Bytecode.Shl;
+    Bytecode.Shr
+  ].
+Proof. repeat econstructor. Qed.
+
+(*
+#[test]
+fn test_or_and_correct_types() {
+    for instr in vec![Bytecode::Or, Bytecode::And] {
+        let code = vec![Bytecode::LdFalse, Bytecode::LdTrue, instr.clone()];
+        let module = make_module(code);
+        let fun_context = get_fun_context(&module);
+        let result = type_safety::verify(&module, &fun_context, &mut DummyMeter);
+        assert!(result.is_ok());
+    }
+}
+*)
+Definition test_or_and_correct_types
+    (instr : Bytecode.t) :
+    M!? PartialVMError.t unit :=
+  let code := [Bytecode.LdFalse; Bytecode.LdTrue; instr] in
+  let module := make_module code in
+  let! fun_context := get_fun_context module in
+  verify module fun_context.
+
+Goal List.Forall
+  (fun instr => test_or_and_correct_types instr = return!? tt)
+  [
+    Bytecode.Or;
+    Bytecode.And
+  ].
+Proof.
+  repeat constructor.
+Qed.
+
+(*
+#[test]
+fn test_or_and_wrong_types() {
+    for instr in vec![Bytecode::Or, Bytecode::And] {
+        let code = vec![Bytecode::LdU32(42), Bytecode::LdTrue, instr.clone()];
+        let module = make_module(code);
+        let fun_context = get_fun_context(&module);
+        let result = type_safety::verify(&module, &fun_context, &mut DummyMeter);
+        assert_eq!(
+            result.unwrap_err().major_status(),
+            StatusCode::BOOLEAN_OP_TYPE_MISMATCH_ERROR
+        );
+
+        let code = vec![Bytecode::LdTrue, Bytecode::LdU64(42), instr.clone()];
+        let module = make_module(code);
+        let fun_context = get_fun_context(&module);
+        let result = type_safety::verify(&module, &fun_context, &mut DummyMeter);
+        assert_eq!(
+            result.unwrap_err().major_status(),
+            StatusCode::BOOLEAN_OP_TYPE_MISMATCH_ERROR
+        );
+    }
+}
+*)
+Definition test_or_and_wrong_types
+    (instr : Bytecode.t) :
+    M! unit :=
+  let code := [Bytecode.LdU32 42; Bytecode.LdTrue; instr] in
+  let module := make_module code in
+  let! fun_context := get_fun_context module in
+  let result := verify module fun_context in
+  do! assert_major_status
+    result
+    (fun status =>
+      match status with
+      | StatusCode.BOOLEAN_OP_TYPE_MISMATCH_ERROR => true
+      | _ => false
+      end
+    ) in
+  let code := [Bytecode.LdTrue; Bytecode.LdU64 42; instr] in
+  let module := make_module code in
+  let! fun_context := get_fun_context module in
+  let result := verify module fun_context in
+  assert_major_status
+    result
+    (fun status =>
+      match status with
+      | StatusCode.BOOLEAN_OP_TYPE_MISMATCH_ERROR => true
+      | _ => false
+      end
+    ).
+
+Goal List.Forall
+  (fun instr => test_or_and_wrong_types instr = return! tt)
+  [
+    Bytecode.Or;
+    Bytecode.And
+  ].
+Proof.
+  repeat constructor.
+Qed.
+
+(*
+#[test]
+#[should_panic]
+fn test_or_and_too_few_args() {
+    for instr in vec![Bytecode::Or, Bytecode::And] {
+        let code = vec![Bytecode::LdTrue, instr.clone()];
+        let module = make_module(code);
+        let fun_context = get_fun_context(&module);
+        let _result = type_safety::verify(&module, &fun_context, &mut DummyMeter);
+    }
+}
+*)
+Definition test_or_and_too_few_args
+    (instr : Bytecode.t) :
+    M!? _ unit :=
+  let code := [Bytecode.LdTrue; instr] in
+  let module := make_module code in
+  let! fun_context := get_fun_context module in
+  verify module fun_context.
+
+Goal List.Forall
+  (fun instr =>
+    exists (Error : Set) (error : Error),
+    test_or_and_too_few_args instr = panic! error
+  )
+  [
+    Bytecode.Or;
+    Bytecode.And
+  ].
+Proof. repeat econstructor. Qed.
+
+(*
+#[test]
+#[should_panic]
+fn test_or_and_no_args() {
+    for instr in vec![Bytecode::Or, Bytecode::And] {
+        let code = vec![instr.clone()];
+        let module = make_module(code);
+        let fun_context = get_fun_context(&module);
+        let _result = type_safety::verify(&module, &fun_context, &mut DummyMeter);
+    }
+}
+*)
+Definition test_or_and_no_args
+    (instr : Bytecode.t) :
+    M!? _ unit :=
+  let code := [instr] in
+  let module := make_module code in
+  let! fun_context := get_fun_context module in
+  verify module fun_context.
+
+Goal List.Forall
+  (fun instr =>
+    exists (Error : Set) (error : Error),
+    test_or_and_no_args instr = panic! error
+  )
+  [
+    Bytecode.Or;
+    Bytecode.And
+  ].
+Proof. repeat econstructor. Qed.
+
+(*
+#[test]
+fn test_not_correct_type() {
+    let code = vec![Bytecode::LdFalse, Bytecode::Not];
+    let module = make_module(code);
+    let fun_context = get_fun_context(&module);
+    let result = type_safety::verify(&module, &fun_context, &mut DummyMeter);
+    assert!(result.is_ok());
+}
+*)
+Definition test_not_correct_type : M!? PartialVMError.t unit :=
+  let code := [Bytecode.LdFalse; Bytecode.Not] in
+  let module := make_module code in
+  let! fun_context := get_fun_context module in
+  verify module fun_context.
+
+Goal test_not_correct_type = return!? tt.
+Proof. reflexivity. Qed.
+
+(*
+#[test]
+fn test_not_wrong_type() {
+    let code = vec![Bytecode::LdU32(42), Bytecode::Not];
+    let module = make_module(code);
+    let fun_context = get_fun_context(&module);
+    let result = type_safety::verify(&module, &fun_context, &mut DummyMeter);
+    assert_eq!(
+        result.unwrap_err().major_status(),
+        StatusCode::BOOLEAN_OP_TYPE_MISMATCH_ERROR
+    );
+}
+*)
+Definition test_not_wrong_type : M! unit :=
+  let code := [Bytecode.LdU32 42; Bytecode.Not] in
+  let module := make_module code in
+  let! fun_context := get_fun_context module in
+  assert_major_status
+    (verify module fun_context)
+    (fun status =>
+      match status with
+      | StatusCode.BOOLEAN_OP_TYPE_MISMATCH_ERROR => true
+      | _ => false
+      end
+    ).
+
+Goal test_not_wrong_type = return! tt.
+Proof. reflexivity. Qed.
+
+(*
+#[test]
+#[should_panic]
+fn test_not_no_arg() {
+    let code = vec![Bytecode::Not];
+    let module = make_module(code);
+    let fun_context = get_fun_context(&module);
+    let _result = type_safety::verify(&module, &fun_context, &mut DummyMeter);
+}
+*)
+Definition test_not_no_arg : M!? _ unit :=
+  let code := [Bytecode.Not] in
+  let module := make_module code in
+  let! fun_context := get_fun_context module in
+  verify module fun_context.
+
+Goal
+  exists (Error : Set) (error : Error),
+  test_not_no_arg = panic! error.
+Proof. repeat eexists. Qed.
+
+(*
+#[test]
+fn test_comparison_correct_types() {
+    for instr in vec![
+        Bytecode::Lt,
+        Bytecode::Gt,
+        Bytecode::Le,
+        Bytecode::Ge,
+        Bytecode::Eq,
+        Bytecode::Neq,
+    ] {
+        for push_ty_instr in vec![
+            Bytecode::LdU8(42),
+            Bytecode::LdU16(257),
+            Bytecode::LdU32(89),
+            Bytecode::LdU64(94),
+            Bytecode::LdU128(Box::new(9999)),
+            Bytecode::LdU256(Box::new(U256::from(745_u32))),
+        ] {
+            let code = vec![push_ty_instr.clone(), push_ty_instr.clone(), instr.clone()];
+            let module = make_module(code);
+            let fun_context = get_fun_context(&module);
+            let result = type_safety::verify(&module, &fun_context, &mut DummyMeter);
+            assert!(result.is_ok());
+        }
+    }
+}
+*)
+Definition test_comparison_correct_types
+    (instr push_ty_instr : Bytecode.t) :
+    M!? PartialVMError.t unit :=
+  let code := [push_ty_instr; push_ty_instr; instr] in
+  let module := make_module code in
+  let! fun_context := get_fun_context module in
+  verify module fun_context.
+
+Goal List.Forall
+  (fun instr =>
+    List.Forall
+      (fun push_ty_instr =>
+        test_comparison_correct_types instr push_ty_instr = return!? tt
+      )
+      [
+        Bytecode.LdU8 42;
+        Bytecode.LdU16 257;
+        Bytecode.LdU32 89;
+        Bytecode.LdU64 94;
+        Bytecode.LdU128 9999;
+        Bytecode.LdU256 745
+      ]
+  )
+  [
+    Bytecode.Lt;
+    Bytecode.Gt;
+    Bytecode.Le;
+    Bytecode.Ge;
+    Bytecode.Eq;
+    Bytecode.Neq
+  ].
+Proof.
+  repeat constructor.
+Qed.
+
+(*
+#[test]
+fn test_comparison_mismatched_types() {
+    for instr in vec![Bytecode::Lt, Bytecode::Gt, Bytecode::Le, Bytecode::Ge] {
+        let code = vec![Bytecode::LdU8(42), Bytecode::LdU64(94), instr.clone()];
+        let module = make_module(code);
+        let fun_context = get_fun_context(&module);
+        let result = type_safety::verify(&module, &fun_context, &mut DummyMeter);
+        assert_eq!(
+            result.unwrap_err().major_status(),
+            StatusCode::INTEGER_OP_TYPE_MISMATCH_ERROR
+        );
+    }
+}
+*)
+Definition test_comparison_mismatched_types
+    (instr : Bytecode.t) :
+    M! unit :=
+  let code := [Bytecode.LdU8 42; Bytecode.LdU64 94; instr] in
+  let module := make_module code in
+  let! fun_context := get_fun_context module in
+  assert_major_status
+    (verify module fun_context)
+    (fun status =>
+      match status with
+      | StatusCode.INTEGER_OP_TYPE_MISMATCH_ERROR => true
+      | _ => false
+      end
+    ).
+
+Goal List.Forall
+  (fun instr => test_comparison_mismatched_types instr = return! tt)
+  [
+    Bytecode.Lt;
+    Bytecode.Gt;
+    Bytecode.Le;
+    Bytecode.Ge
+  ].
+Proof.
+  repeat constructor.
+Qed.
+
+(*
+#[test]
+fn test_comparison_wrong_type() {
+    for instr in vec![Bytecode::Lt, Bytecode::Gt, Bytecode::Le, Bytecode::Ge] {
+        let code = vec![Bytecode::LdTrue, Bytecode::LdU64(94), instr.clone()];
+        let module = make_module(code);
+        let fun_context = get_fun_context(&module);
+        let result = type_safety::verify(&module, &fun_context, &mut DummyMeter);
+        assert_eq!(
+            result.unwrap_err().major_status(),
+            StatusCode::INTEGER_OP_TYPE_MISMATCH_ERROR
+        );
+
+        let code = vec![Bytecode::LdU32(94), Bytecode::LdFalse, instr.clone()];
+        let module = make_module(code);
+        let fun_context = get_fun_context(&module);
+        let result = type_safety::verify(&module, &fun_context, &mut DummyMeter);
+        assert_eq!(
+            result.unwrap_err().major_status(),
+            StatusCode::INTEGER_OP_TYPE_MISMATCH_ERROR
+        );
+    }
+}
+*)
+Definition test_comparison_wrong_type
+    (instr : Bytecode.t) :
+    M! unit :=
+  let code := [Bytecode.LdTrue; Bytecode.LdU64 94; instr] in
+  let module := make_module code in
+  let! fun_context := get_fun_context module in
+  let result := verify module fun_context in
+  do! assert_major_status
+    result
+    (fun status =>
+      match status with
+      | StatusCode.INTEGER_OP_TYPE_MISMATCH_ERROR => true
+      | _ => false
+      end
+    ) in
+  let code := [Bytecode.LdU32 94; Bytecode.LdFalse; instr] in
+  let module := make_module code in
+  let! fun_context := get_fun_context module in
+  let result := verify module fun_context in
+  assert_major_status
+    result
+    (fun status =>
+      match status with
+      | StatusCode.INTEGER_OP_TYPE_MISMATCH_ERROR => true
+      | _ => false
+      end
+    ).
+
+Goal List.Forall
+  (fun instr => test_comparison_wrong_type instr = return! tt)
+  [
+    Bytecode.Lt;
+    Bytecode.Gt;
+    Bytecode.Le;
+    Bytecode.Ge
+  ].
+Proof.
+  repeat constructor.
+Qed.
+
+(*
+#[test]
+#[should_panic]
+fn test_comparison_too_few_args() {
+    for instr in vec![Bytecode::Lt, Bytecode::Gt, Bytecode::Le, Bytecode::Ge] {
+        let code = vec![Bytecode::LdU16(42), instr.clone()];
+        let module = make_module(code);
+        let fun_context = get_fun_context(&module);
+        let _result = type_safety::verify(&module, &fun_context, &mut DummyMeter);
+    }
+}
+*)
+Definition test_comparison_too_few_args
+    (instr : Bytecode.t) :
+    M!? _ unit :=
+  let code := [Bytecode.LdU16 42; instr] in
+  let module := make_module code in
+  let! fun_context := get_fun_context module in
+  verify module fun_context.
+
+Goal List.Forall
+  (fun instr =>
+    exists (Error : Set) (error : Error),
+    test_comparison_too_few_args instr = panic! error
+  )
+  [
+    Bytecode.Lt;
+    Bytecode.Gt;
+    Bytecode.Le;
+    Bytecode.Ge
+  ].
+Proof. repeat econstructor. Qed.
+
+(*
+#[test]
+#[should_panic]
+fn test_comparison_no_args() {
+    for instr in vec![Bytecode::Lt, Bytecode::Gt, Bytecode::Le, Bytecode::Ge] {
+        let code = vec![instr.clone()];
+        let module = make_module(code);
+        let fun_context = get_fun_context(&module);
+        let _result = type_safety::verify(&module, &fun_context, &mut DummyMeter);
+    }
+}
+*)
+Definition test_comparison_no_args
+    (instr : Bytecode.t) :
+    M!? _ unit :=
+  let code := [instr] in
+  let module := make_module code in
+  let! fun_context := get_fun_context module in
+  verify module fun_context.
+
+Goal List.Forall
+  (fun instr =>
+    exists (Error : Set) (error : Error),
+    test_comparison_no_args instr = panic! error
+  )
+  [
+    Bytecode.Lt;
+    Bytecode.Gt;
+    Bytecode.Le;
+    Bytecode.Ge
+  ].
+Proof. repeat econstructor. Qed.
+
+(*
+#[test]
+fn test_branch_nop_ok() {
+    for instr in vec![Bytecode::Branch(0), Bytecode::Nop] {
+        let code = vec![instr];
+        let module = make_module(code);
+        let fun_context = get_fun_context(&module);
+        let result = type_safety::verify(&module, &fun_context, &mut DummyMeter);
+        assert!(result.is_ok());
+    }
+}
+*)
+Definition test_branch_nop_ok
+    (instr : Bytecode.t) :
+    M!? PartialVMError.t unit :=
+  let code := [instr] in
+  let module := make_module code in
+  let! fun_context := get_fun_context module in
+  verify module fun_context.
+
+Goal List.Forall
+  (fun instr => test_branch_nop_ok instr = return!? tt)
+  [
+    Bytecode.Branch 0;
+    Bytecode.Nop
+  ].
+Proof.
+  repeat constructor.
+Qed.
+
+(*
+#[test]
+fn test_ld_integers_ok() {
+    for instr in vec![
+        Bytecode::LdU8(42),
+        Bytecode::LdU16(257),
+        Bytecode::LdU32(89),
+        Bytecode::LdU64(94),
+        Bytecode::LdU128(Box::new(9999)),
+        Bytecode::LdU256(Box::new(U256::from(745_u32))),
+    ] {
+        let code = vec![instr];
+        let module = make_module(code);
+        let fun_context = get_fun_context(&module);
+        let result = type_safety::verify(&module, &fun_context, &mut DummyMeter);
+        assert!(result.is_ok());
+    }
+}
+*)
+Definition test_ld_integers_ok
+    (instr : Bytecode.t) :
+    M!? PartialVMError.t unit :=
+  let code := [instr] in
+  let module := make_module code in
+  let! fun_context := get_fun_context module in
+  verify module fun_context.
+
+Goal List.Forall
+  (fun instr => test_ld_integers_ok instr = return!? tt)
+  [
+    Bytecode.LdU8 42;
+    Bytecode.LdU16 257;
+    Bytecode.LdU32 89;
+    Bytecode.LdU64 94;
+    Bytecode.LdU128 9999;
+    Bytecode.LdU256 745
+  ].
+Proof.
+  repeat constructor.
+Qed.
+
+(*
+#[test]
+fn test_ld_true_false_ok() {
+    for instr in vec![Bytecode::LdTrue, Bytecode::LdFalse] {
+        let code = vec![instr];
+        let module = make_module(code);
+        let fun_context = get_fun_context(&module);
+        let result = type_safety::verify(&module, &fun_context, &mut DummyMeter);
+        assert!(result.is_ok());
+    }
+}
+*)
+Definition test_ld_true_false_ok
+    (instr : Bytecode.t) :
+    M!? PartialVMError.t unit :=
+  let code := [instr] in
+  let module := make_module code in
+  let! fun_context := get_fun_context module in
+  verify module fun_context.
+
+Goal List.Forall
+  (fun instr => test_ld_true_false_ok instr = return!? tt)
+  [
+    Bytecode.LdTrue;
+    Bytecode.LdFalse
+  ].
+Proof.
+  repeat constructor.
+Qed.
+
+(*
+#[test]
+fn test_ld_const_ok() {
+    let code = vec![Bytecode::LdConst(ConstantPoolIndex(0))];
+    let constant = Constant {
+        type_: SignatureToken::U32,
+        data: vec![42, 15, 17, 51],
+    };
+    let mut module: CompiledModule = make_module(code);
+    module.constant_pool.push(constant);
+    assert!(constants::verify_module(&module).is_ok());
+    let fun_context = get_fun_context(&module);
+    let result = type_safety::verify(&module, &fun_context, &mut DummyMeter);
+    assert!(result.is_ok());
+}
+*)
+Definition test_ld_const_ok : M!? PartialVMError.t unit :=
+  let code := [Bytecode.LdConst (ConstantPoolIndex.Build_t 0)] in
+  let constant := {|
+    Constant.type_ := SignatureToken.U32;
+    Constant.data := [42; 15; 17; 51]
+  |} in
+  let module := make_module code in
+  let module := module <|
+    CompiledModule.constant_pool :=
+      module.(CompiledModule.constant_pool) ++ [constant]
+  |> in
+  do! assert_is_ok $ verify_module module in
+  let! fun_context := get_fun_context module in
+  verify module fun_context.
+
+Goal test_ld_const_ok = return!? tt.
+Proof. reflexivity. Qed.
+
+(*
+#[test]
+fn test_pack_correct_types() {
+    let code = vec![
+        Bytecode::LdU32(42),
+        Bytecode::LdTrue,
+        Bytecode::Pack(StructDefinitionIndex(0)),
+    ];
+    let mut module: CompiledModule = make_module(code);
+    add_simple_struct(&mut module);
+    let fun_context = get_fun_context(&module);
+    let result = type_safety::verify(&module, &fun_context, &mut DummyMeter);
+    assert!(result.is_ok());
+}
+*)
+Definition test_pack_correct_types : M!? PartialVMError.t unit :=
+  let code := [
+    Bytecode.LdU32 42;
+    Bytecode.LdTrue;
+    Bytecode.Pack (StructDefinitionIndex.Build_t 0)
+  ] in
+  let module := make_module code in
+  let module := add_simple_struct module in
+  let! fun_context := get_fun_context module in
+  verify module fun_context.
+
+Goal test_pack_correct_types = return!? tt.
+Proof. reflexivity. Qed.
+
+(*
+#[test]
+fn test_pack_mismatched_types() {
+    let code = vec![
+        Bytecode::LdTrue,
+        Bytecode::LdU32(42),
+        Bytecode::Pack(StructDefinitionIndex(0)),
+    ];
+    let mut module: CompiledModule = make_module(code);
+    add_simple_struct(&mut module);
+    let fun_context = get_fun_context(&module);
+    let result = type_safety::verify(&module, &fun_context, &mut DummyMeter);
+    assert_eq!(
+        result.unwrap_err().major_status(),
+        StatusCode::PACK_TYPE_MISMATCH_ERROR
+    );
+}
+*)
+Definition test_pack_mismatched_types : M! unit :=
+  let code := [
+    Bytecode.LdTrue;
+    Bytecode.LdU32 42;
+    Bytecode.Pack (StructDefinitionIndex.Build_t 0)
+  ] in
+  let module := make_module code in
+  let module := add_simple_struct module in
+  let! fun_context := get_fun_context module in
+  assert_major_status
+    (verify module fun_context)
+    (fun status =>
+      match status with
+      | StatusCode.PACK_TYPE_MISMATCH_ERROR => true
+      | _ => false
+      end
+    ).
+
+Goal test_pack_mismatched_types = return! tt.
+Proof. reflexivity. Qed.
+
+(*
+#[test]
+#[should_panic]
+fn test_pack_too_few_args() {
+    let code = vec![Bytecode::LdTrue, Bytecode::Pack(StructDefinitionIndex(0))];
+    let mut module: CompiledModule = make_module(code);
+    add_simple_struct(&mut module);
+    let fun_context = get_fun_context(&module);
+    let _result = type_safety::verify(&module, &fun_context, &mut DummyMeter);
+}
+*)
+Definition test_pack_too_few_args : M!? _ unit :=
+  let code := [Bytecode.LdTrue; Bytecode.Pack (StructDefinitionIndex.Build_t 0)] in
+  let module := make_module code in
+  let module := add_simple_struct module in
+  let! fun_context := get_fun_context module in
+  verify module fun_context.
+
+Goal
+  exists (Error : Set) (error : Error),
+  test_pack_too_few_args = panic! error.
+Proof. repeat eexists. Qed.
+
+(*
+#[test]
+fn test_pack_generic_correct_types() {
+    let code = vec![
+        Bytecode::LdU32(42),
+        Bytecode::PackGeneric(StructDefInstantiationIndex(0)),
+    ];
+    let mut module: CompiledModule = make_module(code);
+    add_simple_struct_generic_with_abilities(
+        &mut module,
+        AbilitySet::PRIMITIVES,
+        SignatureToken::U32,
+    );
+    let fun_context = get_fun_context(&module);
+    let result = type_safety::verify(&module, &fun_context, &mut DummyMeter);
+    assert!(result.is_ok());
+
+    let code = vec![
+        Bytecode::LdU64(42),
+        Bytecode::PackGeneric(StructDefInstantiationIndex(0)),
+    ];
+    let mut module: CompiledModule = make_module(code);
+    add_simple_struct_generic_with_abilities(
+        &mut module,
+        AbilitySet::PRIMITIVES,
+        SignatureToken::U64,
+    );
+    let fun_context = get_fun_context(&module);
+    let result = type_safety::verify(&module, &fun_context, &mut DummyMeter);
+    assert!(result.is_ok());
+}
+*)
+Definition test_pack_generic_correct_types : M!? PartialVMError.t unit :=
+  let code := [
+    Bytecode.LdU32 42;
+    Bytecode.PackGeneric (StructDefInstantiationIndex.Build_t 0)
+  ] in
+  let module := make_module code in
+  let module := add_simple_struct_generic_with_abilities
+    module AbilitySet.PRIMITIVES SignatureToken.U32 in
+  let! fun_context := get_fun_context module in
+  let! result := verify module fun_context in
+  do! assert_is_ok result in
+  let code := [
+    Bytecode.LdU64 42;
+    Bytecode.PackGeneric (StructDefInstantiationIndex.Build_t 0)
+  ] in
+  let module := make_module code in
+  let module := add_simple_struct_generic_with_abilities
+    module AbilitySet.PRIMITIVES SignatureToken.U64 in
+  let! fun_context := get_fun_context module in
+  verify module fun_context.
+
+Goal test_pack_generic_correct_types = return!? tt.
+Proof. reflexivity. Qed.
+
+(*
+#[test]
+fn test_pack_generic_mismatched_types() {
+    let code = vec![
+        Bytecode::LdU64(42),
+        Bytecode::PackGeneric(StructDefInstantiationIndex(0)),
+    ];
+    let mut module: CompiledModule = make_module(code);
+    add_simple_struct_generic_with_abilities(
+        &mut module,
+        AbilitySet::PRIMITIVES,
+        SignatureToken::U32,
+    );
+    let fun_context = get_fun_context(&module);
+    let result = type_safety::verify(&module, &fun_context, &mut DummyMeter);
+    assert_eq!(
+        result.unwrap_err().major_status(),
+        StatusCode::PACK_TYPE_MISMATCH_ERROR
+    );
+}
+*)
+Definition test_pack_generic_mismatched_types : M! unit :=
+  let code := [
+    Bytecode.LdU64 42;
+    Bytecode.PackGeneric (StructDefInstantiationIndex.Build_t 0)
+  ] in
+  let module := make_module code in
+  let module := add_simple_struct_generic_with_abilities
+    module AbilitySet.PRIMITIVES SignatureToken.U32 in
+  let! fun_context := get_fun_context module in
+  assert_major_status
+    (verify module fun_context)
+    (fun status =>
+      match status with
+      | StatusCode.PACK_TYPE_MISMATCH_ERROR => true
+      | _ => false
+      end
+    ).
+
+Goal test_pack_generic_mismatched_types = return! tt.
+Proof. reflexivity. Qed.
+
+(*
+#[test]
+#[should_panic]
+fn test_pack_generic_too_few_args() {
+    let code = vec![Bytecode::PackGeneric(StructDefInstantiationIndex(0))];
+    let mut module: CompiledModule = make_module(code);
+    add_simple_struct_generic_with_abilities(
+        &mut module,
+        AbilitySet::PRIMITIVES,
+        SignatureToken::U32,
+    );
+    let fun_context = get_fun_context(&module);
+    let _result = type_safety::verify(&module, &fun_context, &mut DummyMeter);
+}
+*)
+Definition test_pack_generic_too_few_args : M!? _ unit :=
+  let code := [Bytecode.PackGeneric (StructDefInstantiationIndex.Build_t 0)] in
+  let module := make_module code in
+  let module := add_simple_struct_generic_with_abilities
+    module AbilitySet.PRIMITIVES SignatureToken.U32 in
+  let! fun_context := get_fun_context module in
+  verify module fun_context.
+
+Goal
+  exists (Error : Set) (error : Error),
+  test_pack_generic_too_few_args = panic! error.
+Proof. repeat eexists. Qed.
+
+(*
+#[test]
+fn test_unpack_correct_types() {
+    let code = vec![
+        Bytecode::LdU32(42),
+        Bytecode::LdTrue,
+        Bytecode::Pack(StructDefinitionIndex(0)),
+        Bytecode::Unpack(StructDefinitionIndex(0)),
+    ];
+    let mut module: CompiledModule = make_module(code);
+    add_simple_struct(&mut module);
+    let fun_context = get_fun_context(&module);
+    let result = type_safety::verify(&module, &fun_context, &mut DummyMeter);
+    assert!(result.is_ok());
+}
+*)
+Definition test_unpack_correct_types : M!? PartialVMError.t unit :=
+  let code := [
+    Bytecode.LdU32 42;
+    Bytecode.LdTrue;
+    Bytecode.Pack (StructDefinitionIndex.Build_t 0);
+    Bytecode.Unpack (StructDefinitionIndex.Build_t 0)
+  ] in
+  let module := make_module code in
+  let module := add_simple_struct module in
+  let! fun_context := get_fun_context module in
+  verify module fun_context.
+
+Goal test_unpack_correct_types = return!? tt.
+Proof. reflexivity. Qed.
+
+(*
+#[test]
+fn test_unpack_wrong_type() {
+    let code = vec![
+        Bytecode::LdU32(42),
+        Bytecode::Unpack(StructDefinitionIndex(0)),
+    ];
+    let mut module: CompiledModule = make_module(code);
+    add_simple_struct(&mut module);
+    let fun_context = get_fun_context(&module);
+    let result = type_safety::verify(&module, &fun_context, &mut DummyMeter);
+    assert_eq!(
+        result.unwrap_err().major_status(),
+        StatusCode::UNPACK_TYPE_MISMATCH_ERROR
+    );
+}
+*)
+Definition test_unpack_wrong_type : M! unit :=
+  let code := [
+    Bytecode.LdU32 42;
+    Bytecode.Unpack (StructDefinitionIndex.Build_t 0)
+  ] in
+  let module := make_module code in
+  let module := add_simple_struct module in
+  let! fun_context := get_fun_context module in
+  assert_major_status
+    (verify module fun_context)
+    (fun status =>
+      match status with
+      | StatusCode.UNPACK_TYPE_MISMATCH_ERROR => true
+      | _ => false
+      end
+    ).
+
+Goal test_unpack_wrong_type = return! tt.
+Proof. reflexivity. Qed.
+
+(*
+#[test]
+#[should_panic]
+fn test_unpack_no_arg() {
+    let code = vec![Bytecode::Unpack(StructDefinitionIndex(0))];
+    let mut module: CompiledModule = make_module(code);
+    add_simple_struct(&mut module);
+    let fun_context = get_fun_context(&module);
+    let _result = type_safety::verify(&module, &fun_context, &mut DummyMeter);
+}
+*)
+Definition test_unpack_no_arg : M!? _ unit :=
+  let code := [Bytecode.Unpack (StructDefinitionIndex.Build_t 0)] in
+  let module := make_module code in
+  let module := add_simple_struct module in
+  let! fun_context := get_fun_context module in
+  verify module fun_context.
+
+Goal
+  exists (Error : Set) (error : Error),
+  test_unpack_no_arg = panic! error.
+Proof. repeat eexists. Qed.
