CoqOfRust/move_sui/simulations/move_bytecode_verifier/constants.v
@@ -1,0 +1,86 @@
+Require Import CoqOfRust.CoqOfRust.
+Require coqutil.Datatypes.List.
+Require Import CoqOfRust.simulations.M.
+
+Import simulations.M.Notations.
+
+Require Import CoqOfRust.move_sui.simulations.move_binary_format.errors.
+Require Import CoqOfRust.move_sui.simulations.move_binary_format.file_format.
+Require Import CoqOfRust.move_sui.simulations.move_core_types.vm_status.
+(*
+fn verify_constant_type(idx: usize, type_: &SignatureToken) -> PartialVMResult<()> {
+    if type_.is_valid_for_constant() {
+        Ok(())
+    } else {
+        Err(verification_error(
+            StatusCode::INVALID_CONSTANT_TYPE,
+            IndexKind::ConstantPool,
+            idx as TableIndex,
+        ))
+    }
+}
+*)
+Definition verify_constant_type (idx : Z) (type_ : SignatureToken.t) : PartialVMResult.t unit :=
+  if SignatureToken.is_valid_for_constant type_ then
+    Result.Ok tt
+  else
+    Result.Err (verification_error
+      StatusCode.INVALID_CONSTANT_TYPE
+      IndexKind.ConstantPool
+      idx
+    ).
+
+(*
+fn verify_constant_data(idx: usize, constant: &Constant) -> PartialVMResult<()> {
+    match constant.deserialize_constant() {
+        Some(_) => Ok(()),
+        None => Err(verification_error(
+            StatusCode::MALFORMED_CONSTANT_DATA,
+            IndexKind::ConstantPool,
+            idx as TableIndex,
+        )),
+    }
+}
+*)
+Definition verify_constant_data (idx : Z) (constant : Constant.t) : PartialVMResult.t unit :=
+  (* As we have not implement the deserialization yet, we always return success. *)
+  (* TODO: implement the rest of the function *)
+  Result.Ok tt.
+
+(*
+fn verify_constant(idx: usize, constant: &Constant) -> PartialVMResult<()> {
+    verify_constant_type(idx, &constant.type_)?;
+    verify_constant_data(idx, constant)
+}
+*)
+Definition verify_constant (idx : Z) (constant : Constant.t) : PartialVMResult.t unit :=
+  let? _ := verify_constant_type idx constant.(Constant.type_) in
+  verify_constant_data idx constant.
+
+(*
+fn verify_module_impl(module: &CompiledModule) -> PartialVMResult<()> {
+    for (idx, constant) in module.constant_pool().iter().enumerate() {
+        verify_constant(idx, constant)?
+    }
+    Ok(())
+}
+*)
+Definition verify_module_impl (module : CompiledModule.t) : PartialVMResult.t unit :=
+  fold?
+    tt
+    (List.enumerate 0 module.(CompiledModule.constant_pool))
+    (fun _ '(idx, constant) => verify_constant (Z.of_nat idx) constant).
+
+(*
+pub fn verify_module(module: &CompiledModule) -> VMResult<()> {
+    verify_module_impl(module).map_err(|e| e.finish(Location::Module(module.self_id())))
+}
+*)
+Definition verify_module (module : CompiledModule.t) : VMResult.t unit :=
+  match verify_module_impl module with
+  | Result.Ok _ => Result.Ok tt
+  | Result.Err e =>
+    Result.Err (
+      PartialVMError.finish e (Location.Module (CompiledModule.self_id module))
+    )
+  end.
