CoqOfRust/move_sui/simulations/move_core_types/language_storage.v
@@ -1,0 +1,14 @@
+Require Import CoqOfRust.CoqOfRust.
+Require Import CoqOfRust.simulations.M.
+
+Import simulations.M.Notations.
+
+(*
+pub struct ModuleId {
+    address: AccountAddress,
+    name: Identifier,
+}
+*)
+Module ModuleId.
+  Parameter t : Set.
+End ModuleId.
